Add byte sizes and enforce Remaining Length constraints
Enforcing the `Remaining Length` of the Fixed Header was one of the
first challenges I was thinking about in this project. Initially, I
thought of making a multi-stage solution where we would build packets
with some constraints (stage 0), then run some other constraints against
it (stage 1), then others (stage 2), etc. Computing the Remaining Length
would be a stage 1 constraint. The stage we are in would be enforced
with a GADT using tags for each stage.

The specific Remaining Length problem was more easily fixed with the
`PredType` primitive. We simply add a predicate to the top-level packet
stating "the remaining length must be correct". We enforce this by
implementing `byteSize` for every single primitive, then using these
primitives to build up each component. In the future, we would like to
generate `byteSize` automatically (through `deriving` or some macro) to
facilitate this error-prone process.

LeanMqtt/Core/WithByteSize.lean
@@ -25,6 +25,12 @@ instance instStringByteLength : GetByteSize String where
 instance : GetByteSize (Array UInt8) where
   byteSize := Array.size
 
+@[simp]
+def Unit.byteSize (_ : Unit) : Nat := 0
+
+instance : GetByteSize Unit where
+  byteSize := Unit.byteSize
+
 -- class LengthEmbedding (lenTyp : Type) where
 --   toNat : lenTyp → Nat
 --   injective : Function.Injective toNat
@@ -62,6 +68,21 @@ def WithByteSize.of {α lenTyp} [s : GetByteSize α] [Coe lenTyp Nat]
     (h : s.byteSize val = ↑(OfNat.ofNat (s.byteSize val) : lenTyp) := by rfl) :
     WithByteSize α lenTyp :=
   ⟨val, ⟨OfNat.ofNat (s.byteSize val), h⟩⟩
+
+/--
+`GetByteSize` instance for `WithByteSize`. Recall that `len : lenTyp` is guaranteed to have
+the correct byte size. Thus, the final byte size is the size of `lenTyp` plus the value of `len`.
+-/
+@[simp]
+def WithByteSize.byteSize {α lenTyp : Type}
+    [s_val : GetByteSize α] [s_len : GetByteSize lenTyp] [Coe lenTyp Nat]
+    (w : WithByteSize α lenTyp) : Nat :=
+  s_len.byteSize w.len.val + w.len.val
+
+instance instGetByteSizeWithByteSize
+    {α lenTyp : Type} [s_val : GetByteSize α] [s_len : GetByteSize lenTyp] [Coe lenTyp Nat] :
+    GetByteSize (WithByteSize α lenTyp) where
+  byteSize := WithByteSize.byteSize
 
 /-!
 ### Note on generic binary parser generation (future DSL design)
