LeanMqtt/Packets/Payload/Basic.lean
@@ -1,6 +1,23 @@
+import LeanMqtt.Core.Codec
+import LeanMqtt.Core.WithByteSize
+
 namespace Mqtt
 
 /-- The Payload of an MQTT control packet is currently unimplemented. -/
 structure Payload where
+  -- TODO: Implement Payload variations
+
+def Payload.serialize (_ : Payload) : List UInt8 := []
+def Payload.parser : Parser Payload := pure {}
+
+instance : Codec Payload where
+  serialize := Payload.serialize
+  parser    := Payload.parser
+
+@[simp]
+def Payload.byteSize (_ : Payload) : Nat := 0
+
+instance : GetByteSize Payload where
+  byteSize := Payload.byteSize
 
 end Mqtt
