LeanMqtt/Packets/Proofs.lean
@@ -1,24 +1,27 @@
 import LeanMqtt.Packets.Basic
 import LeanMqtt.Packets.FixedHeader.Proofs
 import LeanMqtt.Packets.VarHeader.Proofs
+import LeanMqtt.Packets.Payload.Proofs
 import LeanMqtt.Helpers.ParserTactics
 
 namespace Mqtt
 
-theorem Header.roundtrip (h : Header) {rest : List UInt8} :
-    Header.parser.run (h.serialize ++ rest) = some (h, rest) := by
-  simp [parser, serialize]
+theorem RawPacket.roundtrip (p : RawPacket) {rest : List UInt8} :
+    RawPacket.parser.run (p.serialize ++ rest) = some (p, rest) := by
+  simp [RawPacket.parser, RawPacket.serialize]
   simp [FixedHeader.roundtrip]
   simp [VarHeader.roundtrip]
+  simp [Payload.roundtrip]
+  exact ⟨{}, trivial⟩
 
-theorem Header.reconstruct {h : Header} {input rest : List UInt8} :
-    Header.parser.run input = some (h, rest) → input = h.serialize ++ rest := by
-
-  simp only [parser, serialize]
+theorem RawPacket.reconstruct {p : RawPacket} {input rest : List UInt8} :
+    RawPacket.parser.run input = some (p, rest) → input = p.serialize ++ rest := by
+  simp only [RawPacket.parser, RawPacket.serialize]
   intro h_run
 
   step_parser h_run → fixVal rest1 h_fixVal
   step_parser h_run → varVal rest2 h_varVal
+  step_parser h_run → payloadVal rest3 h_payloadVal
 
   finish_parser h_run → h_eq
 
@@ -26,9 +29,25 @@ theorem Header.reconstruct {h : Header} {input rest : List UInt8} :
 
   have h_fix_rec := FixedHeader.reconstruct h_fixVal
   have h_var_rec := VarHeader.reconstruct h_varVal
+  have h_payload_rec := Payload.reconstruct h_payloadVal
 
-  rw [h_fix_rec, h_var_rec]
+  rw [h_fix_rec, h_var_rec, h_payload_rec]
 
   simp only [List.append_assoc]
+
+instance : LawfulCodec RawPacket where
+  roundtrip := RawPacket.roundtrip
+  reconstruct := RawPacket.reconstruct
+
+theorem Packet.roundtrip (p : Packet) {rest : List UInt8} :
+    Packet.parser.run (p.serialize ++ rest) = some (p, rest) := by
+  simp [Packet.parser, Packet.serialize]
+  exact PredType.roundtrip p
+
+theorem Packet.reconstruct {p : Packet} {input rest : List UInt8} :
+    Packet.parser.run input = some (p, rest) → input = p.serialize ++ rest := by
+  simp only [Packet.parser, Packet.serialize]
+  intro h
+  exact PredType.reconstruct _ h
 
 end Mqtt
